Main.v
@@ -1,0 +1,13 @@
+Require Import Machine.
+Require Import LinearScan.
+
+Module MyMachine <: Machine.
+
+Definition maxReg := 32.
+
+Lemma registers_exist : maxReg > 0.
+Proof. unfold maxReg. omega. Qed.
+
+End MyMachine.
+
+Module Import LS := MLinearScan MyMachine.
